Started fixing juicy concurrency proofs.

concurrency/JuicyMachineModule.v
@@ -40,4 +40,32 @@ Module THE_JUICY_MACHINE.
   Module JTP:=JuicyMachine.SIG.ThreadPool.
   Import JSEM.JuicyMachineLemmas.
 
+  (* safety with ghost updates *)
+  Definition tp_bupd P tp :=
+    exists tid (cnt : JTP.containsThread tp tid), let phi := JTP.getThreadR cnt in
+    forall c : ghost,
+     joins (ghost_of phi) (ghost_fmap (approx (level phi)) (approx (level phi)) c) ->
+     exists b : ghost,
+       joins b (ghost_fmap (approx (level phi)) (approx (level phi)) c) /\
+       exists phi' : rmap,
+         level phi' = level phi /\
+         resource_at phi' = resource_at phi /\ ghost_of phi' = b /\
+         P (JTP.updThreadR cnt phi').
+
+  Inductive jm_csafe (ge : SEM.G) (st : jmachine_state) (m : mem) : nat -> Prop :=
+  | Safe_0 : jm_csafe ge st m 0
+  | HaltedSafe : forall n : nat,
+                 is_true (ssrbool.isSome (JuicyMachine.halted st)) ->
+                 jm_csafe ge st m n
+  | CoreSafe : forall (tp' : jstate) (m' : mem) (n : nat)
+               (Hstep : JuicyMachine.MachStep ge st m (fst (fst st), nil, tp') m')
+               (Hsafe : tp_bupd (fun tp' => jm_csafe ge (fst (fst st), nil, tp') m' n) tp'),
+               jm_csafe ge st m (S n)
+  | AngelSafe : forall (tp' : jstate) (m' : mem) (n : nat)
+                (Hstep : JuicyMachine.MachStep ge st m
+                  (SCH.schedSkip (fst (fst st)), nil, tp') m')
+                (Hsafe : forall U'' : JuicyMachine.Sch,
+                 tp_bupd (fun tp' => jm_csafe ge (U'', nil, tp') m' n) tp'),
+                jm_csafe ge st m (S n).
+
 End THE_JUICY_MACHINE.
