concurrency/concurrent_machine.v
@@ -39,13 +39,13 @@ Notation WRITE :=
                (mksignature (AST.Tint::AST.Tint::AST.Tint::nil) (Some AST.Tint) cc_default)).
 
 Notation MKLOCK :=
-  (EF_external "makelock" (mksignature (AST.Tint::nil) None cc_default)).
+  (EF_external "makelock" (mksignature (AST.Tptr::nil) None cc_default)).
 Notation FREE_LOCK :=
-  (EF_external "freelock" (mksignature (AST.Tint::nil) None cc_default)).
+  (EF_external "freelock" (mksignature (AST.Tptr::nil) None cc_default)).
 
-Notation LOCK_SIG := (mksignature (AST.Tint::nil) None cc_default).
+Notation LOCK_SIG := (mksignature (AST.Tptr::nil) None cc_default).
 Notation LOCK := (EF_external "acquire" LOCK_SIG).
-Notation UNLOCK_SIG := (mksignature (AST.Tint::nil) None cc_default).
+Notation UNLOCK_SIG := (mksignature (AST.Tptr::nil) None cc_default).
 Notation UNLOCK := (EF_external "release" UNLOCK_SIG).
 
 Module Type EventSig.
