concurrency/erased_machine.v
@@ -87,19 +87,19 @@ Module ErasedMachineShell (SEM:Semantics)  <: ConcurrentMachineSig
          (Hcode: getThreadC cnt0 = Kblocked c)
          (Hat_external: at_external Sem genv c m =
                         Some (LOCK, Vptr b ofs::nil))
-         (Hload: Mem.load Mint32 m b (Int.intval ofs) = Some (Vint Int.one))
-         (Hstore: Mem.store Mint32 m b (Int.intval ofs) (Vint Int.zero) = Some m')
+         (Hload: Mem.load Mint32 m b (Ptrofs.intval ofs) = Some (Vint Int.one))
+         (Hstore: Mem.store Mint32 m b (Ptrofs.intval ofs) (Vint Int.zero) = Some m')
          (Htp': tp' = updThreadC cnt0 (Kresume c Vundef)),
-         ext_step genv cnt0 Hcompat tp' m' (acquire (b, Int.intval ofs) None)
+         ext_step genv cnt0 Hcompat tp' m' (acquire (b, Ptrofs.intval ofs) None)
 
    | step_release :
        forall (tp':thread_pool) c m' b ofs
          (Hcode: getThreadC cnt0 = Kblocked c)
          (Hat_external: at_external Sem genv c m =
                         Some (UNLOCK, Vptr b ofs::nil))
-         (Hstore: Mem.store Mint32 m b (Int.intval ofs) (Vint Int.one) = Some m')
+         (Hstore: Mem.store Mint32 m b (Ptrofs.intval ofs) (Vint Int.one) = Some m')
          (Htp': tp' = updThreadC cnt0 (Kresume c Vundef)),
-         ext_step genv cnt0 Hcompat tp' m' (release (b, Int.intval ofs) None)
+         ext_step genv cnt0 Hcompat tp' m' (release (b, Ptrofs.intval ofs) None)
 
    | step_create :
        forall (tp_upd tp':thread_pool) c b ofs arg
@@ -108,16 +108,16 @@ Module ErasedMachineShell (SEM:Semantics)  <: ConcurrentMachineSig
                         Some (CREATE, Vptr b ofs::arg::nil))
          (Htp_upd: tp_upd = updThreadC cnt0 (Kresume c Vundef))
          (Htp': tp' = addThread tp_upd (Vptr b ofs) arg tt),
-         ext_step genv cnt0 Hcompat tp' m (spawn (b, Int.intval ofs) None None)
+         ext_step genv cnt0 Hcompat tp' m (spawn (b, Ptrofs.intval ofs) None None)
 
    | step_mklock :
        forall  (tp': thread_pool) c m' b ofs
           (Hcode: getThreadC cnt0 = Kblocked c)
           (Hat_external: at_external Sem genv c m =
                          Some (MKLOCK, Vptr b ofs::nil))
-          (Hstore: Mem.store Mint32 m b (Int.intval ofs) (Vint Int.zero) = Some m')
+          (Hstore: Mem.store Mint32 m b (Ptrofs.intval ofs) (Vint Int.zero) = Some m')
           (Htp': tp' = updThreadC cnt0 (Kresume c Vundef)),
-         ext_step genv cnt0 Hcompat tp' m' (mklock (b, Int.intval ofs))
+         ext_step genv cnt0 Hcompat tp' m' (mklock (b, Ptrofs.intval ofs))
 
    | step_freelock :
        forall (tp' tp'': thread_pool) c b ofs
@@ -125,15 +125,15 @@ Module ErasedMachineShell (SEM:Semantics)  <: ConcurrentMachineSig
          (Hat_external: at_external Sem genv c m =
                         Some (FREE_LOCK, Vptr b ofs::nil))
          (Htp': tp' = updThreadC cnt0 (Kresume c Vundef)),
-         ext_step genv cnt0 Hcompat  tp' m (freelock (b,Int.intval ofs))
+         ext_step genv cnt0 Hcompat  tp' m (freelock (b,Ptrofs.intval ofs))
 
    | step_acqfail :
        forall  c b ofs
           (Hcode: getThreadC cnt0 = Kblocked c)
           (Hat_external: at_external Sem genv c m =
                          Some (LOCK, Vptr b ofs::nil))
-          (Hload: Mem.load Mint32 m b (Int.intval ofs) = Some (Vint Int.zero)),
-         ext_step genv cnt0 Hcompat tp m (failacq (b, Int.intval ofs)).
+          (Hload: Mem.load Mint32 m b (Ptrofs.intval ofs) = Some (Vint Int.zero)),
+         ext_step genv cnt0 Hcompat tp m (failacq (b, Ptrofs.intval ofs)).
 
    Definition threadStep (genv : G): forall {tid0 ms m},
        containsThread ms tid0 -> mem_compatible ms m ->
@@ -207,7 +207,7 @@ Module ErasedMachineShell (SEM:Semantics)  <: ConcurrentMachineSig
           erewrite <- gsoThreadCC; eassumption.
         * exists (cntUpdateC (Kresume c Vundef) cnt cntj), q.
           erewrite <- gsoThreadCC; eassumption.
-        * exists (cntRemoveL (b0, Int.intval ofs)
+        * exists (cntRemoveL (b0, Ptrofs.intval ofs)
                         (cntUpdateC (Kresume c Vundef) cnt cntj)), q.
           erewrite <- gsoThreadCC; eassumption.
         * exists cntj, q; assumption.
