sepcomp/simulations_lemmas.v
@@ -67,8 +67,8 @@ Section Eff_INJ_SIMU_DIAGRAMS.
           meminj_preserves_globals ge1 (extern_of mu) /\
           (forall b, isGlobalBlock ge1 b = true -> frgnBlocksSrc mu b = true).
 
-   Hypothesis inj_initial_cores: forall v vals1 c1 m1 j vals2 m2 DomS DomT,
-          initial_core Sem1 0 ge1 m1 v vals1 = Some (c1, None) ->
+   Hypothesis inj_initial_cores: forall v vals1 c1 m1 j vals2 m2 DomS DomT minit m0,
+          initial_core Sem1 0 ge1 minit v vals1 = Some (c1, m0) ->
           Mem.inject j m1 m2 ->
           Forall2 (val_inject j) vals1 vals2 ->
           meminj_preserves_globals ge1 j ->
@@ -86,7 +86,7 @@ Section Eff_INJ_SIMU_DIAGRAMS.
          (forall b, DomT b = true -> Mem.valid_block m2 b) ->
 
        exists c2,
-            initial_core Sem2 0 ge2 m2 v vals2 = Some (c2, None) /\
+            initial_core Sem2 0 ge2 minit v vals2 = Some (c2, m0) /\
             match_states c1 (initial_SM DomS
                                        DomT
                                        (REACH m1 (fun b => isGlobalBlock ge1 b || getBlocks vals1 b))
@@ -221,7 +221,7 @@ clear - match_visible. intros. destruct H; subst. eauto.
 clear - match_validblocks. intros.
     destruct H; subst. eauto.
 clear - inj_initial_cores . intros.
-    destruct (inj_initial_cores _ _ _ _ _ _ _ _ _ H
+    destruct (inj_initial_cores _ _ _ _ _ _ _ _ _ _ _ H
          H0 H1 H2 H3 H4 H5 H6 H7 H8 H9)
     as [c2 [INI MS]].
   exists c1, c2. intuition.
@@ -356,7 +356,7 @@ clear - match_visible. intros. destruct H; subst. eauto.
 clear - match_validblocks. intros.
     destruct H; subst. eauto.
 clear - inj_initial_cores. intros.
-    destruct (inj_initial_cores _ _ _ _ _ _ _ _ _ H H0 H1 H2 H3 H4 H5 H6 H7 H8 H9)
+    destruct (inj_initial_cores _ _ _ _ _ _ _ _ _ _ _ H H0 H1 H2 H3 H4 H5 H6 H7 H8 H9)
     as [c2 [INI MS]].
   exists c1, c2. intuition.
 clear - inj_effcore_diagram genvs_dom_eq.
